compiler/src/compiler/DeadAssignment.v
@@ -1,0 +1,34 @@
+Require Import compiler.util.Common.
+Require Import compiler.FlatImp.
+Require Import Coq.Lists.List. Import ListNotations.
+Require Import bedrock2.Syntax.
+Require Import coqutil.Tactics.fwd.
+Require Import String.
+Require Import compiler.DeadAssignmentDef.
+Require Import bedrock2.MetricLogging.
+
+Local Notation var := String.string (only parsing).
+
+Section WithArguments.
+  Context {width : Z}.
+  Context {BW :  Bitwidth.Bitwidth width }.
+  Context {word :  word width } {word_ok : word.ok word}.
+  Context {env :  map.map string (list var * list var * stmt var) } {env_ok : map.ok env}.
+  Context {mem :  map.map word (Init.Byte.byte : Type) } {mem_ok: map.ok mem}.
+  Context {locals :  map.map string word } {locals_ok: map.ok locals}.
+  Context {ext_spec : Semantics.ExtSpec} {ext_spec_ok: Semantics.ext_spec.ok ext_spec}.
+
+  Local Hint Constructors exec: core.
+(*
+  Lemma deadassignment_correct_aux:
+    forall eH eL,
+       deadassignment_functions eH = Success eL ->
+       forall sH t m mcH lH post,
+       exec eH sH t m lH mcH post ->
+       exec eL (??? sH) t m lH mcH post.
+  Proof.
+    induction 2.
+    (* most cases stay the same *)
+    all: try solve [simpl; eauto].
+  Admitted. *)
+End WithArguments.
