compiler/src/compiler/Pipeline.v
@@ -300,6 +300,42 @@ Section WithWordAndMem.
       - eauto.
     Qed.
 
+    Lemma deadassignment_functions_NoDup: forall funs funs',
+        (forall f argnames retnames body,
+          map.get funs f = Some (argnames, retnames, body) -> NoDup argnames /\ NoDup retnames) ->
+        (deadassignment_functions funs = Success funs') ->
+        forall f argnames retnames body,
+          map.get funs' f = Some (argnames, retnames, body) -> NoDup argnames /\ NoDup retnames.
+    Proof.
+      unfold deadassignment_functions. intros.
+      eapply map.try_map_values_bw in H0.
+      2: { eassumption.  }
+      unfold deadassignment_function in *.
+      fwd.
+      eapply H.
+      eassumption.
+    Qed.
+
+    Lemma deadassignment_correct: phase_correct FlatWithStrVars FlatWithStrVars deadassignment_functions.
+    Proof.
+      unfold FlatWithStrVars.
+      split; cbn.
+      { unfold map.forall_values, ParamsNoDup. intros.
+        destruct v as  ((argnames & retnames) & body).
+        eapply deadassignment_functions_NoDup; try eassumption.
+        intros. specialize H0 with (1 := H2).
+        simpl in H0. assumption.
+      }
+
+      unfold locals_based_call_spec. intros. fwd.
+      pose proof H0 as GI.
+      unfold  deadassignment_functions in GI.
+      eapply map.try_map_values_fw in GI. 2: eassumption.
+      unfold deadassignment_function in GI. fwd.
+      eexists _, _, _, _. split. 1: eassumption. split. 1: eassumption.
+      intros.
+    Admitted.
+
     Lemma regalloc_functions_NoDup: forall funs funs',
         regalloc_functions funs = Success funs' ->
         forall f argnames retnames body,
